Test.IIO.Effect.fst
@@ -1,0 +1,78 @@
+module Test.IIO.Effect
+
+open IO.Free
+open IO.Effect
+open IIO.Effect 
+
+// static_cmd <-- only static default_check
+// pi_static_cmd <-- static default_check + pi_check
+// mixed_cmd <-- static default_check and dynamic pi_check
+// dynamic_cmd <-- dynamic default_check + pi_check
+
+// static_cmd Openfile "../Makefile"
+
+
+let somePi : monitorable_prop = (fun s0 action ->
+  match action with
+  | (| Read, _ |) -> false
+  | _ -> true)
+
+// This fails because it tries to enforce `somePi` statically
+// but `somePi` does not allow any readings, therefore it does
+// not check.
+[@expect_failure]
+let testStatic2 () : IIO unit somePi (fun _ _ _ -> True) =
+  let fd = pi_static_cmd Openfile somePi "../Makefile" in
+  let msg = pi_static_cmd Read somePi fd in
+  pi_static_cmd Close somePi fd
+
+let testStatic1 () : IIO unit somePi (fun _ _ _ -> True) =
+  let fd = pi_static_cmd Openfile somePi "../Makefile" in
+  let msg = mixed_cmd Read somePi fd in
+  pi_static_cmd Close somePi fd
+
+// mixed_cmd Openfile enforces the default precondition statically
+// and the pi dynamically.
+let testMixed1 (pi:monitorable_prop) : IIO unit pi (fun _ _ _ -> True) =
+  let fd = mixed_cmd Openfile pi "../Makefile" in
+  let msg = mixed_cmd Read pi fd in
+  mixed_cmd Close pi fd
+
+[@expect_failure]
+let testMixed2 (pi:monitorable_prop) : IIO unit pi (fun _ _ _ -> True) =
+  let fd = mixed_cmd Openfile pi "../Makefile" in
+  mixed_cmd Close pi fd;
+  let msg = mixed_cmd Read pi fd in
+  ()
+
+// dynamic_cmd Openfile enforces both default precondition
+// and the pi dynamically.
+let testDynMixed1 (pi:monitorable_prop) : IIO unit pi (fun _ _ _ -> True) =
+  let fd = dynamic_cmd Openfile pi "../Makefile" in // fd is fresh, is open
+  let msg = mixed_cmd Read pi fd in
+  mixed_cmd Close pi fd
+
+let testMixed3 (pi:monitorable_prop) : IIO unit pi (fun _ _ _ -> True) =
+  let fd = mixed_cmd Openfile pi "../Makefile" in
+  let msg = mixed_cmd Close pi fd in
+  dynamic_cmd Close pi fd
+
+[@expect_failure]
+let testMixed4 (pi:monitorable_prop) : IIO unit pi (fun _ _ _ -> True) =
+  let fd = mixed_cmd Openfile pi "../Makefile" in
+  dynamic_cmd Close pi fd;
+  let msg = mixed_cmd Read pi fd in
+  ()
+
+// should verify succesfuly, but throw error at runtime
+// because there is a Read fd after a Close.
+let testDyn1 (pi:monitorable_prop) : IIO unit pi (fun _ _ _ -> True)  =
+  let fd = dynamic_cmd Openfile pi "../Makefile" in
+  dynamic_cmd Close pi fd;
+  let msg = dynamic_cmd Read pi fd in
+  ()
+
+let testDyn2 (pi:monitorable_prop) : IIO unit pi (fun _ _ _ -> True) =
+  let fd = dynamic_cmd Openfile pi "../Makefile" in
+  let msg = dynamic_cmd Read pi fd in
+  dynamic_cmd Close pi fd
